Add Section to solve and Refactor code

apps/tc/tc/stdpp/inj_test.v
@@ -1,26 +1,230 @@
-From stdpp Require Import base.
+From elpi.apps.tc Require Import compiler.
+From Coq Require Export Morphisms RelationClasses List Bool Setoid Peano Utf8.
+
+Class Inj {A B} (R : relation A) (S : relation B) (f : A -> B) : Prop :=
+  inj x y : S (f x) (f y) -> R x y.
+Elpi Override TC TC_check Inj.
 Require Import Lia.
-From elpi Require Import elpi.
 
-(* Print Instances Inj. *)
-Check (_ : forall A B C R1 R2 R3 f g _ _, Inj R1 R3 (compose g f)).
-
-Lemma injCompose: forall A B C (f : A -> B) (g : B -> C), 
-Inj eq eq f -> Inj eq eq g -> Inj eq eq (fun a => g (f a)).
-Proof.
-  intros; apply (compose_inj eq eq); easy.
-Qed.
+Generalizable All Variables.
 
 Definition g x := x + 1.
 Definition f (x: nat) := x.
 
-Lemma isInjg : Inj eq eq g.
+Axiom eq1 : relation nat.
+Axiom eq2 : relation nat.
+Axiom eq3 : relation nat.
+
+Lemma isInjg : Inj eq3 eq1 g. Admitted.
+
+Lemma isInjf : Inj eq1 eq3 f. Admitted.
+
+Lemma isInjf_old : Inj eq1 eq2 f. Admitted.
+Lemma isInjg_old : Inj eq2 eq3 g. Admitted.
+
+Lemma isInjinr {A B}: Inj eq eq (@inr A B).
 Proof.
-  red; unfold g; destruct x, y; lia.
+  red; intros.
+  injection H.
+  easy.
 Qed.
 
-Lemma isInjf : Inj eq eq f.
-Proof.
-  red; unfold f; intuition.
+Lemma isInjf_eq : Inj eq eq f.
+Proof. red; intuition. Defined.
+
+Lemma isInjg_eq : Inj eq eq g.
+Proof. red; unfold g; intros [| x] [|y]; lia. Defined.
+
+Global Existing Instance isInjf_eq.
+Global Existing Instance isInjg_eq.
+Global Existing Instance isInjf.
+Global Existing Instance isInjg.
+Global Existing Instance isInjf_old.
+Global Existing Instance isInjg_old.
+Local Instance id_inj {A} : Inj eq eq (@id A).
+Admitted.
+Local Instance inl_inj {A B} : Inj eq eq (@inl A B).
+Admitted.
+Local Instance inr_inj {A B} : Inj eq eq (@inr A B).
+Admitted.
+
+Definition compose {T1 T2 T3: Type} (g: T2 -> T3) (f : T1 -> T2) (x: T1) := g(f x).
+Local Instance compose_inj {A B C} R1 R2 R3 (f : A -> B) (g : B -> C) :
+  Inj R1 R2 f -> Inj R2 R3 g -> Inj R1 R3 (compose g f).
+Admitted.
+
+Elpi add_instances "instances" isInjf_eq isInjg_eq.
+Elpi Print TC_check.
+(* Elpi add_instances Inj. *)
+
+Check (_ : Inj _ _ (compose g f)).
+
+Elpi add_instances Inj.
+
+(* Elpi Debug "debug" "debug ctx->clause" "show-tc-test".  *)
+
+Goal forall (T1 T2 : Type) (f: T1 -> T2) (x : bool), 
+  let r := Inj eq eq f in 
+  let x := true in
+  (if x then r else r) -> r -> Inj eq eq f -> Inj eq eq f.
+  intros.
+  simpl in H.
+  Check (_ : Inj _ _ f).
+Admitted.
+
+Goal forall (T1 T2 : Type) (f: T1 -> T2), 
+  let r := Inj eq eq f in 
+  let b := true in 
+  let cond := (match b with 
+    | true => r 
+    | false => f = f end) in 
+  cond -> Inj eq eq f.
+  intros.
+  unfold cond in H.
+  simpl in H.
+  unfold r in H.
+  Check (_ : Inj _ _ f).
+Admitted.
+
+Section testInj.
+  Context (f : nat -> nat -> nat) `{!Inj eq eq f}.
+
+  Local Instance xxx : Inj eq eq (compose f (Nat.add 3)).
+  Admitted.
+
+  Elpi add_instances Inj.
+  Check (_ : Inj _ _ f).
+  
+  Elpi Print TC_check.
+End testInj.
+
+Elpi Print TC_check.
+
+Class Inj2 {A B C} (R1 : relation A) (R2 : relation B)
+    (S : relation C) (f : A → B → C) : Prop :=
+  inj2 x1 x2 y1 y2 : S (f x1 x2) (f y1 y2) → R1 x1 y1 ∧ R2 x2 y2.
+
+Local Instance inj2_inj_1 `{Inj2 A B C R1 R2 R3 ff} y : Inj R1 R3 (λ x, ff x y).
+Admitted.
+
+Global Instance inj2_inj_2 `{Inj2 A B C R1 R2 R3 ff} x : Inj R2 R3 (ff x).
+Admitted.
+
+Elpi Accumulate TC_check lp:{{
+  :before "hintHook"
+  solve (goal Ctx _ Ty Sol _ as G) GL :-
+    var Sol,
+    % Add's the section's definition to the current context
+    % in order to add its TC if present
+    std.map {coq.env.section} (x\r\ sigma F\ coq.env.typeof (const x) F, r = (decl (global (const x)) _ F)) SectionCtx,
+    ctx->clause {std.append Ctx SectionCtx} Clauses,
+    Clauses => if (tc Ty X) 
+      (
+        refine X G GL ; 
+        coq.say "illtyped solution:" {coq.term->string X}
+      ) 
+      (GL = [seal G]).
+}}.
+Elpi Typecheck TC_check.
+
+Elpi Accumulate tc.db lp:{{
+  :after "complexHook"
+  tc {{ Inj _ _ lp:{{app L}} }} S :- 
+    L = [_, _, _ | _],
+    std.last L Last,
+    std.drop-last 1 L Firsts,
+    tc {{Inj _ _ lp:{{app [app Firsts, Last]}}}} S.
+}}.
+Elpi Typecheck TC_check.
+
+Elpi add_instances Inj Inj2.
+Elpi Typecheck TC_check.
+
+Goal Inj2 eq eq eq Nat.add -> Inj eq eq (Nat.add 0).
+intros.
+apply _.
 Qed.
 
+Generalizable All Variables.
+Class Equiv A := equiv: relation A.
+
+Goal Inj2 eq eq eq Nat.add -> Inj eq eq (fun x => Nat.add x 0).
+intros.
+apply _.
+Qed.
+
+(* Elpi Accumulate TC_check lp:{{
+  :before "hintHook"
+  tc A B :-
+    coq.say "A" A "B" B "End", fail.
+ }}.
+Elpi Typecheck TC_check. *)
+
+(* Elpi Accumulate tc.db lp:{{
+  :after "complexHook"
+  tc {{ Inj _ _ lp:{{app L}} }} S :- 
+    L = [_, _, _ | _],
+    std.last L Last,
+    std.drop-last 1 L Firsts,
+    S = {{@inj2_inj_2 _ _ _ _ _ _ lp:{app Firsts} _ lp:Last}}.
+}}.
+Elpi Typecheck TC_check. *)
+
+
+(* Elpi Accumulate tc.db lp:{{
+  pred prod-len i:term, o:int.
+  prod-len (prod _ _ E) R :-
+    pi x\ sigma X\ prod-len (E x) X, R is X + 1.
+  prod-len _ 1.
+  pred give-len i:term.
+  give-len (prod Name Ty Cnt) :-
+    prod-len Ty Len,
+    coq.say Name Len,
+    pi x\ give-len (Cnt x).
+  give-len _.
+
+  pred compile2 i:term, i:term, i:list (list prop), i:list term, o:prop.
+  compile2 (prod _ T F) CT ListRHS ListVar (pi x\ C x) :-
+    prod-len T Len,
+    coq.say Len,
+    pi p\ sigma L\
+
+      compile2 (F p) CT L [p | ListVar] (C p).
+  compile2 _ I ListRHS ListVar (tc Ty AppInst :- RevRHS) :- 
+    AppInst = app [I | {std.rev ListVar}],
+    std.rev ListRHS RevRHS.
+}}.
+Elpi Typecheck TC_check. *)
+
+Elpi Query TC_check lp:{{
+  coq.locate "Inj" X,
+  const C = X,
+  coq.env.const C _ R.
+  % give-len R.
+}}.
+
+Definition p (T : Type) := @pair T T.
+
+Elpi Print TC_check.
+Goal forall (T1 T2: Set), Inj2 eq eq eq (@p nat) -> Inj eq eq (@p nat 0).
+intros.
+(* apply (inj2_inj_2 ). *)
+apply _.
+Qed.
+
+(* Global Hint Mode Inj - - ! ! -: typeclass_instances.
+Global Hint Mode Inj - - ! ! !: typeclass_instances. *)
+
+(* Elpi add_instances Inj ignoreClasses Inj2 Equiv. *)
+(* Elpi add_instances Inj ignoreInstances isInjf_eq. *)
+(* Elpi add_instances Inj. *)
+(* Elpi add_instances Inj ignoreInstances compose_inj. *)
+(* Elpi add_instances instances compose_inj isInjf_eq isInjg_eq. *)
+(* Elpi add_instances instances inr_inj. *)
+
+Goal forall (A: Type) (x: A -> A), let y := Inj eq eq x in let z := y in z -> Inj eq eq (compose x x).
+Proof.
+  intros T x y z H.
+  (* following diverges: the compiler should unfold the def *)
+  (* Check (_ : Inj eq eq (compose x x)). *)
+Admitted. 
